formal-proofs/LetTick/Soundness.lean
@@ -9,32 +9,28 @@ open ResourceDemand
 theorem soundness (p : Prog) (r_1 r_2 : ResourceDemand) (t : BaseType) 
   : Evaluation p r_1 → Typing p t r_2 → r_2 ≽ r_1 := by 
   intros e_H t_H
-  simp[relaxation_of]; simp[init]; simp[resid]; 
+  simp[relaxation_of];
   cases e_H 
   cases t_H
   rename_i k suff_res
   case _ => {
     apply And.intro
-    have h : init r_2 ≥ k
-    {linarith}
-    . simp[init]; rw[← init]; linarith
     . simp; linarith
+    . simp[suff_res]
   }
   case _ => {
     cases t_H
     rename_i k suff_res
     apply And.intro
     . simp
-    . simp; rw[← init, ← resid]; 
-      have h : |k| ≥ 0
-      {simp}
-      linarith
+    . simp 
   }
   case _ => {
     rename_i e_1 e_2 r_1 r_3 e_1H e_2H 
     apply And.intro
     . simp; 
-    . 
+    . apply [And.intro]
+
   }
 
 
